---
title: Chapter6 plane geometry Module2 triangles lower
lang: en-US
---

| Platforms   | Courses                                                                                      | Coursewares                                                       |
|-------------|----------------------------------------------------------------------------------------------|-------------------------------------------------------------------|
| YouTube     | [Watch](https://www.youtube.com/watch?v=N06rtVZbOeo&list=PLm0MFkgiW1JgKq1kku2WxmrElFbDl7p_s) | [Courseware](../../public/math/Core%20courses/pdf/Courseware.pdf) |
| Dailymotion | [Watch](https://www.dailymotion.com/video/x9gsua6?playlist=x9h6d2)                           |                                                                   |
| Rumble      | [Watch](https://rumble.com/v6s95gn-25-chapter6-plane-geometry-module2-triangles-lower.html)  |                                                                   |


## 14.Right triangle
This can be determined by the Pythagorean theorem $\boxed{a^2+b^2=c^2}$ or by an angle of $\boxed{90^\circ}$.  


## 15.Isosceles right triangle
A right triangle where the three sides are in the ratio $\boxed{1:1:\sqrt{2}}$ or where $\boxed{\text{two sides are equal}}$.


## 16.Equilateral triangle
The three sides are equal, or the three interior angles are equal, or the four centers coincide. 


## 17.Isosceles triangle
A triangle with two equal sides or two equal angles.


## 18.Focus 8
__Triangle identification__  
- The main approach is 
  to use the conditions involving the relationships between the interior angles and the three sides of a triangle, 
  combined with the properties of triangles to determine the shape of the triangle.  
- Focus should be placed on mastering the __characteristics of Equilateral triangles, Isosceles triangles, Right triangles, Isosceles right triangles__.  
- When the given conditions in a problem involve the side lengths of a triangle, the key is to use identity transformations to find the relationships among $a,b,c$.  


::: wrap
### $\fbox{20}\:$The three sides $\small a,b,c$ of $\small \triangle ABC$ satisfy $\small 1+\frac{b}{c}=\frac{b+c}{b+c-a}$, then the triangle is $\small \mathpunct{?}$.
$
\begin{array}{lllll}
(\text{A}) \: \text{An isosceles triangle with side }a\text{ as the leg} &
(\text{B}) \: \text{An isosceles triangle with side }a\text{ as the base} & \\
(\text{C}) \: \text{Equilateral triangle} &
(\text{D}) \: \text{Right triangle} & \\
(\text{E}) \: \text{Obtuse triangle} & \\
\end{array}
$  
:::
#### Solution
::: wrap
$
\begin{array}{ll}
\frac{b+c}{c}=\frac{b+c}{b+c-a} \\
\frac{\cancel{b+c}}{c}=\frac{\cancel{b+c}}{b+c-a}=b+c-a=c & \text{Since condition }a+b>c\text{ satisfied,
the numerator} \ne 0\text{and equal} \\
b=a \\
\end{array}
$  
:::  
#### Conclusion
- Derived Solution  
  ::: wrap
  > $\mathbf{(A)}$  
  > According to the Solution, get $b=a$, so choose $A$. 

  :::
- Formula used  
  ::: wrap
  >$
  \begin{array}{ll}
  a+b>c & \href{/math/0%20Core%20courses/23%20Chapter6%20plane%20geometry%20Module1%20parallel%20lines%20Module2%20triangles%20upper.html#_2-the-relationship-between-the-three-sides-of-a-triangle}{\text{Triangle Inequality theorem}} \\
  \end{array}
  >$

  :::
- Additionally, if the problem is $\frac{b}{c}-1=\frac{b-c}{b+c-a}$  
  ::: wrap
  >$
  \begin{array}{ll}
  \frac{b-c}{c}=\frac{b-c}{b+c-a} \\
  ① \;\, \frac{b-c}{\cancel{c}}=\frac{b-c}{\cancel{b+c-a}} = b-c=0 & \text{Assume that }b-c=0  \\
  ② \;\, \frac{\cancel{b-c}}{c}=\frac{\cancel{b-c}}{b+c-a} = c=b+c-a & \text{Assume that }b-c\ne0  \\
  b=c \lor a=b \\
  \end{array}
  >$

  :::  
---

::: wrap
### $\fbox{21}\:$The three sides of $\small \triangle ABC$ are $\small a,b,c$ and they satisfy $\small 4a^2+4b^2+13c^2-8ac-12bc=0$, then $\small \triangle ABC =\, \mathpunct{?}$.
$
\begin{array}{lllll}
(\text{A}) \: \text{Right triangle} &
(\text{B}) \: \text{Isosceles triangle} &
(\text{C}) \: \text{Equilateral triangle} & \\
(\text{D}) \: \text{Isosceles right triangle} &
(\text{E}) \: \text{Acute triangle} & \\
\end{array}
$  
:::
#### Solution
::: wrap  
- Factoring by grouping into a perfect square form, Non-negative $(x)^2 \ge 0$

  $
  \begin{array}{ll}
  4a^2-8ac+4c^2+4b^2-12bc+9c^2=0 \\
  4(a-c)^2+(2b-3c)^2=0 \\
  a=c \land 2b=3c & (x)^2=0 \\
  \end{array}
  $   
  ![Question triangle figure Q-21 solve-1.svg](../../public/math/Core%20courses/Question%20triangle%20figure%20Q-21%20solve-1.svg)   
:::  
#### Conclusion
- Derived Solution  
  ::: wrap
  > $\mathbf{(B)}$  
  > According to the Solution, get $a=c \land 2b=3c$, so choose $B$. 

  :::
- Formula used  
  ::: wrap
  >$
  \begin{array}{ll}
  (a-b)^2=a^2-2ab+b^2 & \text{Perfect square formula} \\
  \end{array}
  >$

  :::
---

::: wrap
### $\fbox{22}\:$The three sides of $\small \triangle ABC$ are $\small a,b,c$. If $\small a^2+2bc=b^2+2ac=c^2+2ab=27$, then $\small \triangle ABC =\, \mathpunct{?}$. 
$
\begin{array}{lllll}
(\text{A}) \: \text{Isosceles triangle} &
(\text{B}) \: \text{Isosceles right triangle} &
(\text{C}) \: \text{Obtuse triangle} & \\
(\text{D}) \: \text{Right triangle} &
(\text{E}) \: \text{Equilateral triangle} & \\
\end{array}
$  
:::
#### Solution
::: wrap   
$
\begin{array}{ll}
\begin{cases}
a^2+2bc=27 \; ①\\
b^2+2ac=27 \; ②\\
c^2+2ab=27 \; ③\\
\end{cases}
 & \text{} \\
a^2+b^2+c^2+2ab+2ac+2bc=27\times3 & \text{Add all terms together to form a perfect square} \\
(a+b+c)^2=81 \\
a+b+c=\sqrt{81}=9 \\
(a^2+2bc)-(b^2+2ac)=27-27 & ①\,-② \\
a^2-b^2+2bc-2ac=0 \\
(a+b)(a-b)+2c(b-a)=0 \\
(a-b)(a+b-2c)=0 \\
a=b \lor a+b=2c & (0)(a+b-2c)=0 \lor (a-b)(0)=0 \\
a=b
\begin{cases}
a+b+c=9  \\
\boxed{
\begin{array}{ll}
c+2a=9 \;\\
a^2+2ac=27 & ② \;\\
c^2+2a^2=27 & ③ \;\\
(c^2+2a^2)-(a^2+2ac)=27-27 & ③\,-② \;\\
c^2-2ac+a^2=0 \;\\
(c-a)^2=0 \;\\
c=a & (0)^2=0 \;\\
c+2c=9 & a=c \;\\
3c=9 \;\\
c=\frac{9}{3}=3 \;\\
a=b=c=3 \;\\
\end{array}}
\end{cases} \\
a+b=2c
\begin{cases}
a+b+c=9  \\
\boxed{
\begin{array}{ll}
2c+c=9 \;\\
3c=9 \;\\
c=\frac{9}{3}=3 \;\\
a+b=6 \;\\
b^2+6a=27 &  ② \;\; c=3 \;\\
9+2ab=27 & ③ \;\; c=3 \;\\
ab=\frac{18}{2}=9 & ③ \;\\
6 \ge 2\sqrt{9} & a+b \ge 2\sqrt{ab} \;\\
6=6 \Rightarrow \boxed{a=b \land a+b=6} \Rightarrow \boxed{a=b=3} \;\\
a=b=c=3 \;\\
\end{array}}
\end{cases}
\end{array}
$  
:::  
#### Conclusion
- Derived Solution  
  ::: wrap
  > $\mathbf{(E)}$  
  > According to the Solution, get $a=b=c=3$, so choose $E$. 

  :::
- Formula used  
  ::: wrap
  >$
  \begin{array}{ll}
  \begin{cases}
  (a+b)^2=a^2+2ab+b^2 \\
  (a-b)^2=a^2-2ab+b^2
  \end{cases} & \text{Perfect square formula} \\
  a^2-b^2=(a-b)(a+b) & \text{Difference of squares formula} \\
  a+b \ge 2\sqrt{ab} & \text{Arithmetic Mean-Geometric Mean Inequality} \\
  \end{array}
  >$

  :::
---

## 19.Congruence of triangle

### $\textcolor{#1E3A5F}{\fbox{1}}\:$Definition
If two triangles have the __same share and size__, they're said to be congruent. 

### $\textcolor{#1E3A5F}{\fbox{2}}\:$Identification
Congruence can be identified using __side-side-side (SSS),
side-angle-side (SAS), angle-side-angle (ASA), angle-angle-side
(AAS)__.

### $\textcolor{#1E3A5F}{\fbox{3}}\:$Properties
If two triangles are congruent, __their corresponding sides, corresponding angles, and areas are equal__. 
In mathematics terms, the two triangles are equivalent, having the __same side lengths, angles, and areas__.

### $\textcolor{#1E3A5F}{\fbox{4}}\:$Applications
When __folding, symmetry, or rotation__ occurs, congruence analysis can be used.
