---
title: Chapter7 resolve geometry Module3 circle
lang: en-US
---
| Platforms   | Courses                                                                                      | Coursewares                                                       |
|-------------|----------------------------------------------------------------------------------------------|-------------------------------------------------------------------|
| YouTube     | [Watch](https://www.youtube.com/watch?v=Tzz3WDdaVEI&list=PLm0MFkgiW1JgKq1kku2WxmrElFbDl7p_s) | [Courseware](../../public/math/Core%20courses/pdf/Courseware.pdf) |
| Dailymotion | [Watch](https://www.dailymotion.com/video/x9gsui2?playlist=x9h6d2)                           |                                                                   |
| Rumble      | [Watch](https://rumble.com/v6s95hp-29-chapter7-resolve-geometry-module3-circle.html)                                    |                                                                   |



# Module 7–03 Circle

## 1. Equation of a Circle

### $\textcolor{#1E3A5F}{\fbox{1}}\:$Standard Form
- A circle with center $(x_0,y_0)$ and radius $r$ can be represented by the equation: $(x-x_0)^2+(y-y_0)^2=r^2.$
- __Equation derivations__   
  ::: wrap    
  ![Circle standard form derivation.svg](../../public/math/Core%20courses/Circle%20standard%20form%20derivation.svg)  

  $
  \begin{array}{ll}
  \sqrt{(x-x_0)^2+(y-y_0)^2} = r & \href{/math/0%20Core%20courses/27%20Chapter7%20resolve%20geometry%20Module1%20rectangular%20coordinate%20system%20Module2%20straight%20line%20upper.html#_3-distance-formula-between-two-points}{\text{Two-point distance formula}} \\
  (x-x_0)^2+(y-y_0)^2 = r^2 \\
  \text{Example:} \\
  (x+3)^2+(y-2)^2=4 \\
  \text{Center: }(-3,2) & \text{Letting }r=0\text{ makes the circle shrink to a point — the center} \\
  \text{Radius: }r=2 & 2^2=4 \\
  \end{array}
  $  
  :::

### $\textcolor{#1E3A5F}{\fbox{2}}\:$General Form
- $x^2+y^2+ax+by+c=0.$  
- It can be completed into the standard form: $(x+\frac{a}{2})^2+(y+\frac{b}{2})^2=\frac{a^2+b^2-4c}{4}.$  
  - Center: $(-frac{a}{2},-\frac{b}{2}).$
  - Radius: $r=\frac{a^2+b^2-4c}{2}.$
- Note: The condition for the general form to represent a circle is $a^2+b^2-4c>0.$  
- __Equation derivations__   
  ::: wrap    

  $
  \begin{array}{ll}
  (x-x_0)^2+(y-y_0)^2 = r^2 & \text{Standard form} \\
  x^2-2x_0x+x_0^2+y^2-2 y_0y+y_0^2 = r^2 & \text{Expand the perfect square} \\
  x^2+y^2-2x_0x-2y_0y+(x_0^2+y_0^2)=r^2 \\
  x^2+y^2-2x_0x-2y_0y+(x_0^2+y_0^2-r^2)=0 \\
  \text{Let }a=-2x_0 \quad b=-2y_0 \quad c=x_0^2+y_0^2-r^2 \\
  x^2+y^2+ax+by+c=0 \\
  \end{array}
  $  
  :::
